Encrypt Decrypt WIP

src/SDK/EncryptDecrypt.dfy
@@ -40,6 +40,7 @@ module {:extern "EncryptDecrypt"} EncryptDecrypt {
   import Header
   import HeaderTypes
   import HeaderAuth
+  import V1HeaderBody
 
   const DEFAULT_FRAME_LENGTH: uint32 := 4096
 
@@ -88,106 +89,109 @@ module {:extern "EncryptDecrypt"} EncryptDecrypt {
     }
   }
 
-  // Specification of Encrypt with signature
-  function SerializeMessageWithSignature(headerBody: Msg.HeaderBody, headerAuthentication: Msg.HeaderAuthentication, frames: seq<MessageBody.Frame>,
-      signature: seq<uint8>): (message: seq<uint8>)
-    requires forall frame: MessageBody.Frame | frame in frames :: frame.Valid()
-    requires headerBody.Valid()
+  // // Specification of Encrypt with signature
+  function method SerializeMessageWithSignature(
+    framedMessage: MessageBody.FramedMessage,
+    signature: seq<uint8>
+  )
+    :(message: seq<uint8>)
     requires |signature| < UINT16_LIMIT
   {
     var serializedSignature := UInt16ToSeq(|signature| as uint16) + signature;
-    SerializeMessageWithoutSignature(headerBody, headerAuthentication, frames) + serializedSignature
+    SerializeMessageWithoutSignature(framedMessage) + serializedSignature
   }
 
-  // Specification of Encrypt without signature
-  function SerializeMessageWithoutSignature(headerBody: Msg.HeaderBody, headerAuthentication: Msg.HeaderAuthentication,frames: seq<MessageBody.Frame>):
-      (message: seq<uint8>)
-    requires forall frame: MessageBody.Frame | frame in frames :: frame.Valid()
-    requires headerBody.Valid()
+  // // Specification of Encrypt without signature
+  function method SerializeMessageWithoutSignature(
+    framedMessage: MessageBody.FramedMessage
+  )
+    :(message: seq<uint8>)
   {
-    var serializedHeaderBody := (reveal Msg.HeaderBodyToSeq(); Msg.HeaderBodyToSeq(headerBody));
-    var serializedHeaderAuthentication := headerAuthentication.iv + headerAuthentication.authenticationTag;
-    var serializedFrames := MessageBody.FramesToSequence(frames);
-    serializedHeaderBody + serializedHeaderAuthentication + serializedFrames
+    // The header
+    framedMessage.finalFrame.header.rawHeader
+    // The header authentication
+    + HeaderAuth.WriteAESMac(framedMessage.finalFrame.header.headerAuth)
+    // The message body i.e. "all the frames"
+    + MessageBody.WriteFramedMessageBody(framedMessage)
   }
 
-  // Specification of headerBody in Encrypt
-  predicate ValidHeaderBodyForRequest(headerBody: Msg.HeaderBody, request: EncryptRequest)
-  {
-    && headerBody.Valid()
-    && headerBody.version == Msg.VERSION_1
-    && headerBody.typ == Msg.TYPE_CUSTOMER_AED
-    // TODO This is currently failing. What is it proving and is it needed?
-    // && (exists material: Crypto.EncryptionMaterials | DefaultCMMDef.EncryptionMaterialsSignature(material) ::
-    // headerBody.algorithmSuiteID == AlgorithmSuite.PolymorphIDToInternalID(material.algorithmSuiteId)
-    // && headerBody.aad == material.encryptionContext
-    // && headerBody.encryptedDataKeys == Msg.EncryptedDataKeys(material.encryptedDataKeys))
-    && headerBody.contentType == Msg.ContentType.Framed
-    && headerBody.frameLength == if request.frameLength.Some? then request.frameLength.value else DEFAULT_FRAME_LENGTH
-  }
+  // // Specification of headerBody in Encrypt
+  // predicate ValidHeaderBodyForRequest(headerBody: Msg.HeaderBody, request: EncryptRequest)
+  // {
+  //   && headerBody.Valid()
+  //   && headerBody.version == Msg.VERSION_1
+  //   && headerBody.typ == Msg.TYPE_CUSTOMER_AED
+  //   // TODO This is currently failing. What is it proving and is it needed?
+  //   // && (exists material: Crypto.EncryptionMaterials | DefaultCMMDef.EncryptionMaterialsSignature(material) ::
+  //   // headerBody.algorithmSuiteID == AlgorithmSuite.PolymorphIDToInternalID(material.algorithmSuiteId)
+  //   // && headerBody.aad == material.encryptionContext
+  //   // && headerBody.encryptedDataKeys == Msg.EncryptedDataKeys(material.encryptedDataKeys))
+  //   && headerBody.contentType == Msg.ContentType.Framed
+  //   && headerBody.frameLength == if request.frameLength.Some? then request.frameLength.value else DEFAULT_FRAME_LENGTH
+  // }
 
-  // Specification of headerAuthentication in Encrypt
-  predicate ValidHeaderAuthenticationForRequest(headerAuthentication: Msg.HeaderAuthentication, headerBody: Msg.HeaderBody)
-    requires headerBody.Valid()
-  {
-    var serializedHeaderBody := (reveal Msg.HeaderBodyToSeq(); Msg.HeaderBodyToSeq(headerBody));
-    var suite := Client.SpecificationClient().GetSuite(SerializableTypes.GetAlgorithmSuiteId(headerBody.algorithmSuiteID));
-    && headerAuthentication.iv == seq(suite.encrypt.ivLength, _ => 0)
-    && Msg.HeaderAuthenticationMatchesHeaderBody(headerAuthentication, headerBody)
-    && exists encryptionOutput: AESEncryption.EncryptionOutput, cipherkey: seq<uint8> |
-      IsDerivedKey(cipherkey) :: AESEncryption.EncryptedWithKey(encryptionOutput.cipherText, cipherkey)
-  }
+  // // Specification of headerAuthentication in Encrypt
+  // predicate ValidHeaderAuthenticationForRequest(headerAuthentication: Msg.HeaderAuthentication, headerBody: Msg.HeaderBody)
+  //   requires headerBody.Valid()
+  // {
+  //   var serializedHeaderBody := (reveal Msg.HeaderBodyToSeq(); Msg.HeaderBodyToSeq(headerBody));
+  //   var suite := Client.SpecificationClient().GetSuite(SerializableTypes.GetAlgorithmSuiteId(headerBody.algorithmSuiteID));
+  //   && headerAuthentication.iv == seq(suite.encrypt.ivLength, _ => 0)
+  //   && Msg.HeaderAuthenticationMatchesHeaderBody(headerAuthentication, headerBody)
+  //   && exists encryptionOutput: AESEncryption.EncryptionOutput, cipherkey: seq<uint8> |
+  //     IsDerivedKey(cipherkey) :: AESEncryption.EncryptedWithKey(encryptionOutput.cipherText, cipherkey)
+  // }
 
-  // Specification of the Frames used in Encrypt
-  predicate ValidFramesForRequest(frames: seq<MessageBody.Frame>, request: EncryptRequest, headerBody: Msg.HeaderBody)
-  {
-    (forall frame: MessageBody.Frame | frame in frames :: frame.Valid()) //This predicates ensure that the frame can be converted to a sequence
-    && MessageBody.FramesEncryptPlaintext(frames, request.plaintext) // This requirement is missing in spec but needed for now needs to be addapted to match streaming
-    && var suite := Client.SpecificationClient().GetSuite(SerializableTypes.GetAlgorithmSuiteId(headerBody.algorithmSuiteID));
-    && (forall frame: MessageBody.Frame | frame in frames :: |frame.iv| == suite.encrypt.ivLength as int)
-    && (exists cipherkey | IsDerivedKey(cipherkey) :: // The cipherkey used in the encryption is the derived key
-       (forall frame: MessageBody.Frame | frame in frames :: AESEncryption.EncryptedWithKey(frame.encContent, cipherkey)))
-  }
+  // // Specification of the Frames used in Encrypt
+  // predicate ValidFramesForRequest(frames: seq<MessageBody.Frame>, request: EncryptRequest, headerBody: Msg.HeaderBody)
+  // {
+  //   (forall frame: MessageBody.Frame | frame in frames :: frame.Valid()) //This predicates ensure that the frame can be converted to a sequence
+  //   && MessageBody.FramesEncryptPlaintext(frames, request.plaintext) // This requirement is missing in spec but needed for now needs to be addapted to match streaming
+  //   && var suite := Client.SpecificationClient().GetSuite(SerializableTypes.GetAlgorithmSuiteId(headerBody.algorithmSuiteID));
+  //   && (forall frame: MessageBody.Frame | frame in frames :: |frame.iv| == suite.encrypt.ivLength as int)
+  //   && (exists cipherkey | IsDerivedKey(cipherkey) :: // The cipherkey used in the encryption is the derived key
+  //      (forall frame: MessageBody.Frame | frame in frames :: AESEncryption.EncryptedWithKey(frame.encContent, cipherkey)))
+  // }
 
-  //Specification of the Signature used in Encrypt
-  predicate ValidSignatureForRequest(signature: seq<uint8>, headerBody: Msg.HeaderBody, headerAuthentication: Msg.HeaderAuthentication,frames: seq<MessageBody.Frame>)
-    requires forall frame: MessageBody.Frame | frame in frames :: frame.Valid()
-    requires headerBody.Valid()
-  {
-    var serializedMessage := SerializeMessageWithoutSignature(headerBody, headerAuthentication, frames);
-    |signature| < UINT16_LIMIT
-    && (exists material: Crypto.EncryptionMaterials | material.signingKey.Some? ::
-        Signature.IsSigned(material.signingKey.value, serializedMessage, signature))
-  }
+  // //Specification of the Signature used in Encrypt
+  // predicate ValidSignatureForRequest(signature: seq<uint8>, headerBody: Msg.HeaderBody, headerAuthentication: Msg.HeaderAuthentication,frames: seq<MessageBody.Frame>)
+  //   requires forall frame: MessageBody.Frame | frame in frames :: frame.Valid()
+  //   requires headerBody.Valid()
+  // {
+  //   var serializedMessage := SerializeMessageWithoutSignature(headerBody, headerAuthentication, frames);
+  //   |signature| < UINT16_LIMIT
+  //   && (exists material: Crypto.EncryptionMaterials | material.signingKey.Some? ::
+  //       Signature.IsSigned(material.signingKey.value, serializedMessage, signature))
+  // }
 
  /*
   * Encrypt a plaintext and serialize it into a message.
   */
   method Encrypt(request: EncryptRequest)
-      returns (res: Result<seq<uint8>, string>,
-               ghost successSupportingInfo: Option<(Msg.HeaderBody, Msg.HeaderAuthentication, seq<MessageBody.Frame>, seq<uint8>)>)
+      returns (res: Result<seq<uint8>, string>)
+              //  ,ghost successSupportingInfo: Option<(Msg.HeaderBody, Msg.HeaderAuthentication, seq<MessageBody.Frame>, seq<uint8>)>)
     ensures request.cmm == null && request.keyring == null ==> res.Failure?
     ensures request.cmm != null && request.keyring != null ==> res.Failure?
     ensures request.frameLength.Some? && request.frameLength.value == 0 ==> res.Failure?
-    ensures match res
-      case Failure(e) => true
-      case Success(encryptedSequence) =>
-        && successSupportingInfo.Some?
-        && var Some((headerBody, headerAuthentication, frames, signature)) := successSupportingInfo;
-        // The result is a serialization of 3 items with a potential fourth item.
-        // Every item has to meet some specification which is specified in its respective section
-        && ValidHeaderBodyForRequest(headerBody, request) // Which meet their respective specifications
-        && ValidHeaderAuthenticationForRequest(headerAuthentication, headerBody)
-        && ValidFramesForRequest(frames, request, headerBody)
-        && match Client.SpecificationClient().GetSuite(SerializableTypes.GetAlgorithmSuiteId(headerBody.algorithmSuiteID)).signature {
-            case ECDSA(_) => // If the result needs to be signed then there exists a fourth item
-              && ValidSignatureForRequest(signature, headerBody, headerAuthentication, frames) // which meets its specification
-              && encryptedSequence == SerializeMessageWithSignature(headerBody, headerAuthentication, frames, signature) // These items can be serialized to the output
-            case None => // if the result does not need to be signed
-              encryptedSequence == SerializeMessageWithoutSignature(headerBody, headerAuthentication, frames) // Then these items can be serialized to the output
-          }
+    // ensures match res
+    //   case Failure(e) => true
+    //   case Success(encryptedSequence) =>
+    //     && successSupportingInfo.Some?
+    //     && var Some((headerBody, headerAuthentication, frames, signature)) := successSupportingInfo;
+    //     // The result is a serialization of 3 items with a potential fourth item.
+    //     // Every item has to meet some specification which is specified in its respective section
+    //     && ValidHeaderBodyForRequest(headerBody, request) // Which meet their respective specifications
+    //     && ValidHeaderAuthenticationForRequest(headerAuthentication, headerBody)
+    //     && ValidFramesForRequest(frames, request, headerBody)
+    //     && match Client.SpecificationClient().GetSuite(SerializableTypes.GetAlgorithmSuiteId(headerBody.algorithmSuiteID)).signature {
+    //         case ECDSA(_) => // If the result needs to be signed then there exists a fourth item
+    //           && ValidSignatureForRequest(signature, headerBody, headerAuthentication, frames) // which meets its specification
+    //           && encryptedSequence == SerializeMessageWithSignature(headerBody, headerAuthentication, frames, signature) // These items can be serialized to the output
+    //         case None => // if the result does not need to be signed
+    //           encryptedSequence == SerializeMessageWithoutSignature(headerBody, headerAuthentication, frames) // Then these items can be serialized to the output
+    //       }
   {
-    successSupportingInfo := None; // KRML: why is the type of "successSupportingInfo" subject to definite-assignment rules?
+    // successSupportingInfo := None; // KRML: why is the type of "successSupportingInfo" subject to definite-assignment rules?
     // Validate encrypt request
     :- Need(request.cmm != null || request.keyring != null, "EncryptRequest.cmm OR EncryptRequest.keyring must be set.");
     :- Need(!(request.cmm != null && request.keyring != null), "EncryptRequest.keyring AND EncryptRequest.cmm must not both be set.");
@@ -232,20 +236,17 @@ module {:extern "EncryptDecrypt"} EncryptDecrypt {
 
     var esdkId := SerializableTypes.GetESDKAlgorithmSuiteId(encMat.algorithmSuiteId);
     var suite := Client.SpecificationClient().GetSuite(encMat.algorithmSuiteId);
-    var messageID: Msg.MessageID :- Random.GenerateBytes(Msg.MESSAGE_ID_LEN as int32);
+    var messageID: HeaderTypes.MessageID :- Random.GenerateBytes(HeaderTypes.MESSAGE_ID_LEN as int32);
     var derivedDataKey := DeriveKey(encMat.plaintextDataKey.value, suite, messageID);
-
-
-
 
     var body := HeaderTypes.HeaderBody.V1HeaderBody(
       messageType := HeaderTypes.MessageType.TYPE_CUSTOMER_AED,
       esdkSuiteId := esdkId,
       messageId := messageID,
-      encryptionContext :=[], // encMat.encryptionContext,
+      encryptionContext := EncryptionContext.GetCanonicalEncryptionContext(encMat.encryptionContext),
       encryptedDataKeys := encryptedDataKeys,
       contentType := HeaderTypes.ContentType.Framed,
-      headerIvLength := suite.encrypt.ivLength as uint8,
+      headerIvLength := suite.encrypt.ivLength as nat,
       frameLength := frameLength
     );
 
@@ -258,9 +259,10 @@ module {:extern "EncryptDecrypt"} EncryptDecrypt {
       headerAuthTag := encryptionOutput.authTag
     );
 
-    var header : Header := HeaderInfo(
+    var header : Header.Header := Header.HeaderInfo(
       body := body,
       rawHeader := Header.WriteHeaderBody(body),
+      encryptionContext := encMat.encryptionContext,
       suite := suite,
       headerAuth := headerAuth
     );
@@ -276,51 +278,54 @@ module {:extern "EncryptDecrypt"} EncryptDecrypt {
     // var _ :- Serialize.SerializeHeaderAuthentication(wr, headerAuthentication);
     // assert wr.GetDataWritten() == serializedHeaderBody + serializedHeaderAuthentication; // Read data contains complete header
 
-    assert {:focus} true;
-    // Encrypt the given plaintext into the message body and add a footer with a signature, if required
-    var seqWithGhostFrames :- MessageBody.EncryptMessageBody(
+    // assert {:focus} true;
+    // Encrypt the given plaintext into the framed message
+    var framedMessage :- MessageBody.EncryptMessageBody(
       request.plaintext,
       header,
       derivedDataKey
     );
-    var body := seqWithGhostFrames.sequence;
-    ghost var frames := seqWithGhostFrames.frames;
 
-    assert ValidFramesForRequest(frames, request, headerBody) && body == MessageBody.FramesToSequence(frames) by { // Frames meets specification
-      assert {:focus} true;
-      assert forall frame: MessageBody.Frame | frame in frames :: frame.Valid();
-      assert MessageBody.FramesEncryptPlaintext(frames, request.plaintext); // This requirement is missing in spec but needed
-      assert forall frame: MessageBody.Frame | frame in frames :: |frame.iv| == suite.encrypt.ivLength as int;
-      assert IsDerivedKey(derivedDataKey);
-      assert forall frame: MessageBody.Frame | frame in frames :: AESEncryption.EncryptedWithKey(frame.encContent, derivedDataKey);
-    }
+    // var body := seqWithGhostFrames.sequence;
+    // ghost var frames := seqWithGhostFrames.frames;
 
-    var msg := wr.GetDataWritten() + body;
-    if suite.signature.ECDSA? {
+    // assert ValidFramesForRequest(frames, request, headerBody) && body == MessageBody.FramesToSequence(frames) by { // Frames meets specification
+    //   assert {:focus} true;
+    //   assert forall frame: MessageBody.Frame | frame in frames :: frame.Valid();
+    //   assert MessageBody.FramesEncryptPlaintext(frames, request.plaintext); // This requirement is missing in spec but needed
+    //   assert forall frame: MessageBody.Frame | frame in frames :: |frame.iv| == suite.encrypt.ivLength as int;
+    //   assert IsDerivedKey(derivedDataKey);
+    //   assert forall frame: MessageBody.Frame | frame in frames :: AESEncryption.EncryptedWithKey(frame.encContent, derivedDataKey);
+    // }
+
+    // var msg := wr.GetDataWritten() + body;
+    if framedMessage.finalFrame.header.suite.signature.ECDSA? {
+      var msg := SerializeMessageWithoutSignature(framedMessage);
       var ecdsaParams := suite.signature.curve;
       var bytes :- Signature.Sign(ecdsaParams, encMat.signingKey.value, msg);
       :- Need(|bytes| == ecdsaParams.SignatureLength() as int, "Malformed response from Sign().");
 
       var signature := UInt16ToSeq(|bytes| as uint16) + bytes;
-      assert ValidSignatureForRequest(bytes, headerBody, headerAuthentication, frames) by { // Signature confirms to specification
-        assert |signature| < UINT16_LIMIT;
-        assert Signature.IsSigned(encMat.signingKey.value, msg, bytes);
-      }
+      // assert ValidSignatureForRequest(bytes, headerBody, headerAuthentication, frames) by { // Signature confirms to specification
+      //   assert |signature| < UINT16_LIMIT;
+      //   assert Signature.IsSigned(encMat.signingKey.value, msg, bytes);
+      // }
       msg := msg + signature;
-      assert msg == SerializeMessageWithSignature(headerBody, headerAuthentication, frames, bytes); // Header, frames and signature can be serialized into the stream
-      return Success(msg), Some((headerBody, headerAuthentication, frames, bytes));
+      assert msg == SerializeMessageWithSignature(framedMessage, signature); // Header, frames and signature can be serialized into the stream
+      return Success(msg); //, Some((headerBody, headerAuthentication, frames, bytes));
     } else {
-      assert {:focus} true;
+      // assert {:focus} true;
       // don't use a footer
-      assert msg == SerializeMessageWithoutSignature(headerBody, headerAuthentication, frames); // Header and frames can be serialized into the stream
-      return Success(msg), Some((headerBody, headerAuthentication, frames, []));
+      // assert msg == SerializeMessageWithoutSignature(headerBody, headerAuthentication, frames); // Header and frames can be serialized into the stream
+      var msg := SerializeMessageWithoutSignature(framedMessage);
+      return Success(msg); //, Some((headerBody, headerAuthentication, frames, []));
     }
   }
 
   method DeriveKey(
     plaintextDataKey: seq<uint8>,
     suite: Client.AlgorithmSuites.AlgorithmSuite,
-    messageID: Msg.MessageID
+    messageID: HeaderTypes.MessageID
   ) 
     returns (derivedDataKey: seq<uint8>)
     requires |plaintextDataKey| == suite.encrypt.keyLength as int
@@ -349,223 +354,223 @@ module {:extern "EncryptDecrypt"} EncryptDecrypt {
     true
   }
 
-  method Decrypt(request: DecryptRequest) returns (res: Result<seq<uint8>, string>)
-    ensures request.cmm == null && request.keyring == null ==> res.Failure?
-    ensures request.cmm != null && request.keyring != null ==> res.Failure?
-  {
-    var decryptWithVerificationInfo :- DecryptWithVerificationInfo(request);
-    return Success(decryptWithVerificationInfo.plaintext);
-  }
+  // method Decrypt(request: DecryptRequest) returns (res: Result<seq<uint8>, string>)
+  //   ensures request.cmm == null && request.keyring == null ==> res.Failure?
+  //   ensures request.cmm != null && request.keyring != null ==> res.Failure?
+  // {
+  //   var decryptWithVerificationInfo :- DecryptWithVerificationInfo(request);
+  //   return Success(decryptWithVerificationInfo.plaintext);
+  // }
 
   datatype DecryptResultWithVerificationInfo = DecryptResultWithVerificationInfo(
           plaintext: seq<uint8>,
-    ghost header: Msg.Header,
+    ghost header: Header.Header,
     ghost hbSeq: seq<uint8>,
     ghost frames: seq<MessageBody.Frame>,
     ghost signature: Option<seq<uint8>>)
 
 
-  // Verification of this method requires verification of the CMM to some extent, The verification of the Decrypt method should be extended after CMM is verified
-  method DecryptWithVerificationInfo(request: DecryptRequest) returns (res: Result<DecryptResultWithVerificationInfo, string>)
-    ensures request.cmm == null && request.keyring == null ==> res.Failure?
-    ensures request.cmm != null && request.keyring != null ==> res.Failure?
-    ensures match res // Verify that if no error occurs the correct objects are deserialized from the stream
-      case Failure(e) => true
-      case Success(d) => // Unfold return value into seperate variables
-        && d.header.body.Valid()
-        && Msg.IsSerializationOfHeaderBody(d.hbSeq, d.header.body)
-        && (d.header.body.contentType.Framed? ==> // We only verify framed content for now
-          && (forall frame: MessageBody.Frame | frame in d.frames :: frame.Valid())
-          && MessageBody.FramesEncryptPlaintext(d.frames, d.plaintext)
-          && match d.signature {
-               case Some(_) =>
-                 && |d.signature.value| < UINT16_LIMIT
-                 && request.message == d.hbSeq + d.header.auth.iv + d.header.auth.authenticationTag // These items can be serialized to the output
-                   + MessageBody.FramesToSequence(d.frames) + UInt16ToSeq(|d.signature.value| as uint16) + d.signature.value
-               case None => // if the result does not need to be signed
-                 request.message == d.hbSeq + d.header.auth.iv + d.header.auth.authenticationTag + MessageBody.FramesToSequence(d.frames)
-             })
-  {
-    // Validate decrypt request
-    :- Need(request.cmm == null || request.keyring == null, "DecryptRequest.keyring OR DecryptRequest.cmm must be set (not both).");
-    :- Need(request.cmm != null || request.keyring != null, "DecryptRequest.cmm and DecryptRequest.keyring cannot both be null.");
+  // // Verification of this method requires verification of the CMM to some extent, The verification of the Decrypt method should be extended after CMM is verified
+  // method DecryptWithVerificationInfo(request: DecryptRequest) returns (res: Result<DecryptResultWithVerificationInfo, string>)
+  //   ensures request.cmm == null && request.keyring == null ==> res.Failure?
+  //   ensures request.cmm != null && request.keyring != null ==> res.Failure?
+  //   ensures match res // Verify that if no error occurs the correct objects are deserialized from the stream
+  //     case Failure(e) => true
+  //     case Success(d) => // Unfold return value into seperate variables
+  //       && d.header.body.Valid()
+  //       && Msg.IsSerializationOfHeaderBody(d.hbSeq, d.header.body)
+  //       && (d.header.body.contentType.Framed? ==> // We only verify framed content for now
+  //         && (forall frame: MessageBody.Frame | frame in d.frames :: frame.Valid())
+  //         && MessageBody.FramesEncryptPlaintext(d.frames, d.plaintext)
+  //         && match d.signature {
+  //              case Some(_) =>
+  //                && |d.signature.value| < UINT16_LIMIT
+  //                && request.message == d.hbSeq + d.header.auth.iv + d.header.auth.authenticationTag // These items can be serialized to the output
+  //                  + MessageBody.FramesToSequence(d.frames) + UInt16ToSeq(|d.signature.value| as uint16) + d.signature.value
+  //              case None => // if the result does not need to be signed
+  //                request.message == d.hbSeq + d.header.auth.iv + d.header.auth.authenticationTag + MessageBody.FramesToSequence(d.frames)
+  //            })
+  // {
+  //   // Validate decrypt request
+  //   :- Need(request.cmm == null || request.keyring == null, "DecryptRequest.keyring OR DecryptRequest.cmm must be set (not both).");
+  //   :- Need(request.cmm != null || request.keyring != null, "DecryptRequest.cmm and DecryptRequest.keyring cannot both be null.");
 
-    var cmm: Crypto.ICryptographicMaterialsManager;
-    if request.keyring == null {
-      cmm := request.cmm;
-    } else {
-      var client := new Client.AwsCryptographicMaterialProvidersClient();
-      cmm := client
-        .CreateDefaultCryptographicMaterialsManager(Crypto.CreateDefaultCryptographicMaterialsManagerInput(
-        keyring := request.keyring
-      ));
-    }
+  //   var cmm: Crypto.ICryptographicMaterialsManager;
+  //   if request.keyring == null {
+  //     cmm := request.cmm;
+  //   } else {
+  //     var client := new Client.AwsCryptographicMaterialProvidersClient();
+  //     cmm := client
+  //       .CreateDefaultCryptographicMaterialsManager(Crypto.CreateDefaultCryptographicMaterialsManagerInput(
+  //       keyring := request.keyring
+  //     ));
+  //   }
 
-    var rd := new Streams.ByteReader(request.message);
-    var deserializeHeaderResult :- Deserialize.DeserializeHeader(rd);
-    var header := deserializeHeaderResult.header;
-    assert header.body.Valid();
+  //   var rd := new Streams.ByteReader(request.message);
+  //   var deserializeHeaderResult :- Deserialize.DeserializeHeader(rd);
+  //   var header := deserializeHeaderResult.header;
+  //   assert header.body.Valid();
 
-    if header.body.contentType.Framed? { // If the header is framed then the header is deserialized from the read sequence
-      assert HeaderBySequence(header, deserializeHeaderResult.hbSeq, rd.reader.data[..rd.reader.pos]) by {
-        reveal HeaderBySequence();
-        assert header.body.contentType.Framed?;
-        assert header.body.Valid();
-        assert Msg.IsSerializationOfHeaderBody(deserializeHeaderResult.hbSeq, header.body);
-        assert rd.reader.data[..rd.reader.pos] == deserializeHeaderResult.hbSeq + header.auth.iv + header.auth.authenticationTag;
-      }
-      assert DataIsFramed(request.message) by { // Predicate that holds in DataIsFramed this predicate is currently not used but is very usefull for future validation
-        assert 0 <= rd.reader.pos <= |request.message|;
-        assert rd.reader.data[..rd.reader.pos] == request.message[..rd.reader.pos];
-        assert HeaderBySequence(header, deserializeHeaderResult.hbSeq, request.message[..rd.reader.pos]);
-      }
-    }
+  //   if header.body.contentType.Framed? { // If the header is framed then the header is deserialized from the read sequence
+  //     assert HeaderBySequence(header, deserializeHeaderResult.hbSeq, rd.reader.data[..rd.reader.pos]) by {
+  //       reveal HeaderBySequence();
+  //       assert header.body.contentType.Framed?;
+  //       assert header.body.Valid();
+  //       assert Msg.IsSerializationOfHeaderBody(deserializeHeaderResult.hbSeq, header.body);
+  //       assert rd.reader.data[..rd.reader.pos] == deserializeHeaderResult.hbSeq + header.auth.iv + header.auth.authenticationTag;
+  //     }
+  //     assert DataIsFramed(request.message) by { // Predicate that holds in DataIsFramed this predicate is currently not used but is very usefull for future validation
+  //       assert 0 <= rd.reader.pos <= |request.message|;
+  //       assert rd.reader.data[..rd.reader.pos] == request.message[..rd.reader.pos];
+  //       assert HeaderBySequence(header, deserializeHeaderResult.hbSeq, request.message[..rd.reader.pos]);
+  //     }
+  //   }
 
-    var decMatRequest := Crypto.DecryptMaterialsInput(
-      algorithmSuiteId:=SerializableTypes.GetAlgorithmSuiteId(header.body.algorithmSuiteID),
-      encryptedDataKeys:=header.body.encryptedDataKeys,
-      encryptionContext:=header.body.aad);
-    var output :- cmm.DecryptMaterials(decMatRequest);
-    var decMat := output.decryptionMaterials;
+  //   var decMatRequest := Crypto.DecryptMaterialsInput(
+  //     algorithmSuiteId:=SerializableTypes.GetAlgorithmSuiteId(header.body.algorithmSuiteID),
+  //     encryptedDataKeys:=header.body.encryptedDataKeys,
+  //     encryptionContext:=header.body.aad);
+  //   var output :- cmm.DecryptMaterials(decMatRequest);
+  //   var decMat := output.decryptionMaterials;
 
-    // Validate decryption materials
-    :- Need(Client.Materials.DecryptionMaterialsWithPlaintextDataKey(decMat), "CMM returned invalid DecryptMaterials");
-    // Same as with the Encryption Materials, I assert that this is equivalent. Let's talk in the PR!
-    // :- Need(decMat.plaintextDataKey.Some?, "CMM failed to acquire plaintext data key.");
-    // :- Need(|decMat.plaintextDataKey.value| == AlgorithmSuite.PolymorphIDToInternalID(decMat.algorithmSuiteId).KDFInputKeyLength(),
-    //   "CMM return invalid plaintext data key for algorithm suite in use.");
-    // :- Need(AlgorithmSuite.PolymorphIDToInternalID(decMat.algorithmSuiteId).SignatureType().Some? ==> decMat.verificationKey.Some?,
-    //   "CMM failed to acquire verification key.");
+  //   // Validate decryption materials
+  //   :- Need(Client.Materials.DecryptionMaterialsWithPlaintextDataKey(decMat), "CMM returned invalid DecryptMaterials");
+  //   // Same as with the Encryption Materials, I assert that this is equivalent. Let's talk in the PR!
+  //   // :- Need(decMat.plaintextDataKey.Some?, "CMM failed to acquire plaintext data key.");
+  //   // :- Need(|decMat.plaintextDataKey.value| == AlgorithmSuite.PolymorphIDToInternalID(decMat.algorithmSuiteId).KDFInputKeyLength(),
+  //   //   "CMM return invalid plaintext data key for algorithm suite in use.");
+  //   // :- Need(AlgorithmSuite.PolymorphIDToInternalID(decMat.algorithmSuiteId).SignatureType().Some? ==> decMat.verificationKey.Some?,
+  //   //   "CMM failed to acquire verification key.");
 
-    var suite := Client.SpecificationClient().GetSuite(decMat.algorithmSuiteId);
+  //   var suite := Client.SpecificationClient().GetSuite(decMat.algorithmSuiteId);
 
-    var decryptionKey := DeriveKey(decMat.plaintextDataKey.value, suite, header.body.messageID);
+  //   var decryptionKey := DeriveKey(decMat.plaintextDataKey.value, suite, header.body.messageID);
 
-    ghost var endHeaderPos := rd.reader.pos;
-    // Parse and decrypt the message body
-    var plaintext;
-    match header.body.contentType {
-      case NonFramed =>
-        plaintext :- MessageBody.DecryptNonFramedMessageBody(rd, suite, decryptionKey, header.body.messageID);
-      case Framed =>
-        plaintext :- MessageBody.DecryptFramedMessageBody(rd, suite, decryptionKey, header.body.frameLength as int, header.body.messageID);
-    }
+  //   ghost var endHeaderPos := rd.reader.pos;
+  //   // Parse and decrypt the message body
+  //   var plaintext;
+  //   match header.body.contentType {
+  //     case NonFramed =>
+  //       plaintext :- MessageBody.DecryptNonFramedMessageBody(rd, suite, decryptionKey, header.body.messageID);
+  //     case Framed =>
+  //       plaintext :- MessageBody.DecryptFramedMessageBody(rd, suite, decryptionKey, header.body.frameLength as int, header.body.messageID);
+  //   }
 
-    // Ghost variable contains frames which are deserialized from the data read after the header if the data is framed
-    assert header.body.contentType.Framed? ==>
-      exists frames: seq<MessageBody.Frame> | |frames| < UINT32_LIMIT && (forall frame | frame in frames :: frame.Valid())
-        && MessageBody.FramesToSequence(frames) == rd.reader.data[endHeaderPos..rd.reader.pos] ::
-          && MessageBody.FramesEncryptPlaintext(frames, plaintext);
-    ghost var frames: seq<MessageBody.Frame> :| header.body.contentType.Framed? ==>
-        && |frames| < UINT32_LIMIT
-        && (forall frame | frame in frames :: frame.Valid())
-        && MessageBody.FramesToSequence(frames) == rd.reader.data[endHeaderPos..rd.reader.pos]
-        && MessageBody.FramesEncryptPlaintext(frames, plaintext);
+  //   // Ghost variable contains frames which are deserialized from the data read after the header if the data is framed
+  //   assert header.body.contentType.Framed? ==>
+  //     exists frames: seq<MessageBody.Frame> | |frames| < UINT32_LIMIT && (forall frame | frame in frames :: frame.Valid())
+  //       && MessageBody.FramesToSequence(frames) == rd.reader.data[endHeaderPos..rd.reader.pos] ::
+  //         && MessageBody.FramesEncryptPlaintext(frames, plaintext);
+  //   ghost var frames: seq<MessageBody.Frame> :| header.body.contentType.Framed? ==>
+  //       && |frames| < UINT32_LIMIT
+  //       && (forall frame | frame in frames :: frame.Valid())
+  //       && MessageBody.FramesToSequence(frames) == rd.reader.data[endHeaderPos..rd.reader.pos]
+  //       && MessageBody.FramesEncryptPlaintext(frames, plaintext);
 
-    if header.body.contentType.Framed? {
-      assert FramesBySequence(frames, rd.reader.data[endHeaderPos..rd.reader.pos]) by {
-        reveal FramesBySequence();
-        assert |frames| < UINT32_LIMIT;
-        assert forall frame | frame in frames :: frame.Valid();
-        assert rd.reader.data[endHeaderPos..rd.reader.pos] == MessageBody.FramesToSequence(frames);
-      }
-      assert HeaderBySequence(header, deserializeHeaderResult.hbSeq, rd.reader.data[..endHeaderPos]) by {
-        assert endHeaderPos == |deserializeHeaderResult.hbSeq| + |header.auth.iv + header.auth.authenticationTag|;
-        assert HeaderBySequence(header, deserializeHeaderResult.hbSeq, rd.reader.data[..endHeaderPos]);
-      }
-      assert FramesBySequence(frames, rd.reader.data[endHeaderPos..rd.reader.pos]);
-    }
+  //   if header.body.contentType.Framed? {
+  //     assert FramesBySequence(frames, rd.reader.data[endHeaderPos..rd.reader.pos]) by {
+  //       reveal FramesBySequence();
+  //       assert |frames| < UINT32_LIMIT;
+  //       assert forall frame | frame in frames :: frame.Valid();
+  //       assert rd.reader.data[endHeaderPos..rd.reader.pos] == MessageBody.FramesToSequence(frames);
+  //     }
+  //     assert HeaderBySequence(header, deserializeHeaderResult.hbSeq, rd.reader.data[..endHeaderPos]) by {
+  //       assert endHeaderPos == |deserializeHeaderResult.hbSeq| + |header.auth.iv + header.auth.authenticationTag|;
+  //       assert HeaderBySequence(header, deserializeHeaderResult.hbSeq, rd.reader.data[..endHeaderPos]);
+  //     }
+  //     assert FramesBySequence(frames, rd.reader.data[endHeaderPos..rd.reader.pos]);
+  //   }
 
-    ghost var signature: Option<seq<uint8>> := None;
-    ghost var endFramePos := rd.reader.pos;
-    assert header.body.contentType.Framed? ==> 0 <= endHeaderPos <= endFramePos <= |request.message|;
-    if suite.signature.ECDSA? {
-      var verifyResult, locSig := VerifySignature(rd, decMat);
-      signature := Some(locSig);
-      if verifyResult.Failure? {
-        return Failure(verifyResult.error);
-      }
-      assert SignatureBySequence(signature.value, rd.reader.data[endFramePos..rd.reader.pos]); // Read signature from the sequence
-    }
+  //   ghost var signature: Option<seq<uint8>> := None;
+  //   ghost var endFramePos := rd.reader.pos;
+  //   assert header.body.contentType.Framed? ==> 0 <= endHeaderPos <= endFramePos <= |request.message|;
+  //   if suite.signature.ECDSA? {
+  //     var verifyResult, locSig := VerifySignature(rd, decMat);
+  //     signature := Some(locSig);
+  //     if verifyResult.Failure? {
+  //       return Failure(verifyResult.error);
+  //     }
+  //     assert SignatureBySequence(signature.value, rd.reader.data[endFramePos..rd.reader.pos]); // Read signature from the sequence
+  //   }
 
-    var isDone := rd.IsDoneReading();
-    :- Need(isDone, "message contains additional bytes at end");
+  //   var isDone := rd.IsDoneReading();
+  //   :- Need(isDone, "message contains additional bytes at end");
 
-    // Combine gathered facts and convert to postcondition
-    if header.body.contentType.Framed? {
-      if suite.signature.ECDSA? { // Case with Signature
-        assert signature.Some?;
-        assert SignatureBySequence(signature.value, rd.reader.data[endFramePos..rd.reader.pos]);
-        assert HeaderBySequence(header, deserializeHeaderResult.hbSeq, request.message[..endHeaderPos])
-          && FramesBySequence(frames, request.message[endHeaderPos..endFramePos])
-          && SignatureBySequence(signature.value, request.message[endFramePos..]) by {
-            assert 0 <= endHeaderPos <= endFramePos <= |request.message|;
-            assert SignatureBySequence(signature.value, request.message[endFramePos..]) by {
-            assert header.body.contentType.Framed? ==> SignatureBySequence(signature.value, rd.reader.data[endFramePos..rd.reader.pos]);
-            assert rd.reader.data[endFramePos..rd.reader.pos] == request.message[endFramePos..] by {
-              calc {
-                rd.reader.data[endFramePos..rd.reader.pos];
-              == {UpperBoundRemv(rd.reader.data, endFramePos); assert rd.reader.pos == |rd.reader.data|; }
-                rd.reader.data[endFramePos..];
-              == {assert rd.reader.data == request.message; }
-                request.message[endFramePos..];
-              }
-            }
-            assert SignatureBySequence(signature.value, rd.reader.data[endFramePos..rd.reader.pos]);
-          }
-        }
-        HBandMBwithSigMatchSequence(header, deserializeHeaderResult.hbSeq, frames, signature.value, request.message);
-      } else { // Case without signature
-        assert signature.None?;
-        assert 0 <= endHeaderPos <= |request.message| by {
-          assert request.message == rd.reader.data;
-        }
-        assert HeaderBySequence(header, deserializeHeaderResult.hbSeq, request.message[..endHeaderPos])
-          && FramesBySequence(frames, request.message[endHeaderPos..]) by {
-            assert HeaderBySequence(header, deserializeHeaderResult.hbSeq, rd.reader.data[..endHeaderPos])
-              && FramesBySequence(frames, rd.reader.data[endHeaderPos..rd.reader.pos]);
-            assert rd.reader.data[endHeaderPos..rd.reader.pos] == request.message[endHeaderPos..] by {
-              calc {
-                rd.reader.data[endHeaderPos..rd.reader.pos];
-              == {UpperBoundRemv(rd.reader.data, endHeaderPos); }
-                rd.reader.data[endHeaderPos..];
-              == {assert rd.reader.data == request.message; }
-                request.message[endHeaderPos..];
-              }
-            }
-          }
-        assert 0 <= endHeaderPos <= |request.message|;
-        HBandMBMatchSequence(header, deserializeHeaderResult.hbSeq, frames, request.message);
-      }
-    }
-    var decryptResultWithVerificationInfo := DecryptResultWithVerificationInfo(plaintext, header, deserializeHeaderResult.hbSeq, frames, signature);
-    ghost var d := decryptResultWithVerificationInfo;
-    assert d.header.body.Valid();
-    assert Msg.IsSerializationOfHeaderBody(d.hbSeq, d.header.body);
-    if d.header.body.contentType.Framed? {
-      assert forall frame: MessageBody.Frame | frame in d.frames :: frame.Valid();
-      assert MessageBody.FramesEncryptPlaintext(d.frames, d.plaintext);
-      assert match d.signature {
-               case Some(_) =>
-                 && |d.signature.value| < UINT16_LIMIT
-                 && request.message == d.hbSeq + d.header.auth.iv + d.header.auth.authenticationTag // These items can be serialized to the output
-                   + MessageBody.FramesToSequence(d.frames) + UInt16ToSeq(|d.signature.value| as uint16) + d.signature.value
-               case None => // if the result does not need to be signed
-                 request.message == d.hbSeq + d.header.auth.iv + d.header.auth.authenticationTag + MessageBody.FramesToSequence(d.frames)
-             } by
-      {
-        if d.signature.Some? {
-          assert |d.signature.value| < UINT16_LIMIT;
-          assert request.message ==
-                   d.hbSeq + d.header.auth.iv + d.header.auth.authenticationTag // These items can be serialized to the output
-                   + MessageBody.FramesToSequence(d.frames) + UInt16ToSeq(|d.signature.value| as uint16) + d.signature.value;
-        } else {
-          assert request.message == d.hbSeq + d.header.auth.iv + d.header.auth.authenticationTag + MessageBody.FramesToSequence(d.frames);
-        }
-      }
-    }
-    return Success(decryptResultWithVerificationInfo);
-  }
+  //   // Combine gathered facts and convert to postcondition
+  //   if header.body.contentType.Framed? {
+  //     if suite.signature.ECDSA? { // Case with Signature
+  //       assert signature.Some?;
+  //       assert SignatureBySequence(signature.value, rd.reader.data[endFramePos..rd.reader.pos]);
+  //       assert HeaderBySequence(header, deserializeHeaderResult.hbSeq, request.message[..endHeaderPos])
+  //         && FramesBySequence(frames, request.message[endHeaderPos..endFramePos])
+  //         && SignatureBySequence(signature.value, request.message[endFramePos..]) by {
+  //           assert 0 <= endHeaderPos <= endFramePos <= |request.message|;
+  //           assert SignatureBySequence(signature.value, request.message[endFramePos..]) by {
+  //           assert header.body.contentType.Framed? ==> SignatureBySequence(signature.value, rd.reader.data[endFramePos..rd.reader.pos]);
+  //           assert rd.reader.data[endFramePos..rd.reader.pos] == request.message[endFramePos..] by {
+  //             calc {
+  //               rd.reader.data[endFramePos..rd.reader.pos];
+  //             == {UpperBoundRemv(rd.reader.data, endFramePos); assert rd.reader.pos == |rd.reader.data|; }
+  //               rd.reader.data[endFramePos..];
+  //             == {assert rd.reader.data == request.message; }
+  //               request.message[endFramePos..];
+  //             }
+  //           }
+  //           assert SignatureBySequence(signature.value, rd.reader.data[endFramePos..rd.reader.pos]);
+  //         }
+  //       }
+  //       HBandMBwithSigMatchSequence(header, deserializeHeaderResult.hbSeq, frames, signature.value, request.message);
+  //     } else { // Case without signature
+  //       assert signature.None?;
+  //       assert 0 <= endHeaderPos <= |request.message| by {
+  //         assert request.message == rd.reader.data;
+  //       }
+  //       assert HeaderBySequence(header, deserializeHeaderResult.hbSeq, request.message[..endHeaderPos])
+  //         && FramesBySequence(frames, request.message[endHeaderPos..]) by {
+  //           assert HeaderBySequence(header, deserializeHeaderResult.hbSeq, rd.reader.data[..endHeaderPos])
+  //             && FramesBySequence(frames, rd.reader.data[endHeaderPos..rd.reader.pos]);
+  //           assert rd.reader.data[endHeaderPos..rd.reader.pos] == request.message[endHeaderPos..] by {
+  //             calc {
+  //               rd.reader.data[endHeaderPos..rd.reader.pos];
+  //             == {UpperBoundRemv(rd.reader.data, endHeaderPos); }
+  //               rd.reader.data[endHeaderPos..];
+  //             == {assert rd.reader.data == request.message; }
+  //               request.message[endHeaderPos..];
+  //             }
+  //           }
+  //         }
+  //       assert 0 <= endHeaderPos <= |request.message|;
+  //       HBandMBMatchSequence(header, deserializeHeaderResult.hbSeq, frames, request.message);
+  //     }
+  //   }
+  //   var decryptResultWithVerificationInfo := DecryptResultWithVerificationInfo(plaintext, header, deserializeHeaderResult.hbSeq, frames, signature);
+  //   ghost var d := decryptResultWithVerificationInfo;
+  //   assert d.header.body.Valid();
+  //   assert Msg.IsSerializationOfHeaderBody(d.hbSeq, d.header.body);
+  //   if d.header.body.contentType.Framed? {
+  //     assert forall frame: MessageBody.Frame | frame in d.frames :: frame.Valid();
+  //     assert MessageBody.FramesEncryptPlaintext(d.frames, d.plaintext);
+  //     assert match d.signature {
+  //              case Some(_) =>
+  //                && |d.signature.value| < UINT16_LIMIT
+  //                && request.message == d.hbSeq + d.header.auth.iv + d.header.auth.authenticationTag // These items can be serialized to the output
+  //                  + MessageBody.FramesToSequence(d.frames) + UInt16ToSeq(|d.signature.value| as uint16) + d.signature.value
+  //              case None => // if the result does not need to be signed
+  //                request.message == d.hbSeq + d.header.auth.iv + d.header.auth.authenticationTag + MessageBody.FramesToSequence(d.frames)
+  //            } by
+  //     {
+  //       if d.signature.Some? {
+  //         assert |d.signature.value| < UINT16_LIMIT;
+  //         assert request.message ==
+  //                  d.hbSeq + d.header.auth.iv + d.header.auth.authenticationTag // These items can be serialized to the output
+  //                  + MessageBody.FramesToSequence(d.frames) + UInt16ToSeq(|d.signature.value| as uint16) + d.signature.value;
+  //       } else {
+  //         assert request.message == d.hbSeq + d.header.auth.iv + d.header.auth.authenticationTag + MessageBody.FramesToSequence(d.frames);
+  //       }
+  //     }
+  //   }
+  //   return Success(decryptResultWithVerificationInfo);
+  // }
 
   method VerifySignature(rd: Streams.ByteReader, decMat: Crypto.DecryptionMaterials) returns (res: Result<(), string>, ghost signature: seq<uint8>)
     requires rd.Valid()
@@ -607,20 +612,20 @@ module {:extern "EncryptDecrypt"} EncryptDecrypt {
     return Success(()), sigResult.value;
   }
 
-  predicate {:opaque } HeaderBySequence(header: Msg.Header, hbSeq: seq<uint8>, sequence: seq<uint8>)
-  {
-    && header.body.contentType.Framed?
-    && header.body.Valid()
-    && Msg.IsSerializationOfHeaderBody(hbSeq, header.body)
-    && sequence == hbSeq + header.auth.iv + header.auth.authenticationTag
-  }
+  // predicate {:opaque } HeaderBySequence(header: Msg.Header, hbSeq: seq<uint8>, sequence: seq<uint8>)
+  // {
+  //   && header.body.contentType.Framed?
+  //   && header.body.Valid()
+  //   && Msg.IsSerializationOfHeaderBody(hbSeq, header.body)
+  //   && sequence == hbSeq + header.auth.iv + header.auth.authenticationTag
+  // }
 
-  predicate {:opaque } FramesBySequence(frames: seq<MessageBody.Frame>, sequence: seq<uint8>)
-  {
-    && |frames| < UINT32_LIMIT
-    && (forall frame: MessageBody.Frame | frame in frames :: frame.Valid())
-    && sequence == MessageBody.FramesToSequence(frames)
-  }
+  // predicate {:opaque } FramesBySequence(frames: seq<MessageBody.Frame>, sequence: seq<uint8>)
+  // {
+  //   && |frames| < UINT32_LIMIT
+  //   && (forall frame: MessageBody.Frame | frame in frames :: frame.Valid())
+  //   && sequence == MessageBody.FramesToSequence(frames)
+  // }
 
   predicate {:opaque } SignatureBySequence(signature: seq<uint8>, sequence: seq<uint8>)
   {
@@ -628,29 +633,29 @@ module {:extern "EncryptDecrypt"} EncryptDecrypt {
     && sequence == UInt16ToSeq(|signature| as uint16) + signature
   }
 
-  lemma HBandMBMatchSequence(header: Msg.Header, hbSeq: seq<uint8>, frames: seq<MessageBody.Frame>, message: seq<uint8>)
-    requires forall frame: MessageBody.Frame | frame in frames :: frame.Valid()
-    requires |message| >= |hbSeq| + |header.auth.iv + header.auth.authenticationTag|
-    requires exists headerLength | 0 <= headerLength <= |message| ::
-      && HeaderBySequence(header, hbSeq, message[..headerLength])
-      && FramesBySequence(frames, message[headerLength..])
-    ensures message == hbSeq + header.auth.iv + header.auth.authenticationTag + MessageBody.FramesToSequence(frames);
-  {
-    reveal HeaderBySequence(), FramesBySequence();
-  }
+  // lemma HBandMBMatchSequence(header: Msg.Header, hbSeq: seq<uint8>, frames: seq<MessageBody.Frame>, message: seq<uint8>)
+  //   requires forall frame: MessageBody.Frame | frame in frames :: frame.Valid()
+  //   requires |message| >= |hbSeq| + |header.auth.iv + header.auth.authenticationTag|
+  //   requires exists headerLength | 0 <= headerLength <= |message| ::
+  //     && HeaderBySequence(header, hbSeq, message[..headerLength])
+  //     && FramesBySequence(frames, message[headerLength..])
+  //   ensures message == hbSeq + header.auth.iv + header.auth.authenticationTag + MessageBody.FramesToSequence(frames);
+  // {
+  //   reveal HeaderBySequence(), FramesBySequence();
+  // }
 
-  lemma HBandMBwithSigMatchSequence(header: Msg.Header, hbSeq: seq<uint8>, frames: seq<MessageBody.Frame>, signature: seq<uint8>, message: seq<uint8>)
-    requires forall frame: MessageBody.Frame | frame in frames :: frame.Valid()
-    requires |message| >= |hbSeq| + |header.auth.iv + header.auth.authenticationTag| + |MessageBody.FramesToSequence(frames)|
-    requires exists headerLength, frameLength | 0 <= headerLength <= frameLength < |message| ::
-      && HeaderBySequence(header, hbSeq, message[..headerLength])
-      && FramesBySequence(frames, message[headerLength..frameLength])
-      && SignatureBySequence(signature, message[frameLength..])
-    ensures |signature| < UINT16_LIMIT &&
-      message == hbSeq + header.auth.iv + header.auth.authenticationTag + MessageBody.FramesToSequence(frames) + UInt16ToSeq(|signature| as uint16) + signature;
-  {
-    reveal HeaderBySequence(), FramesBySequence(), SignatureBySequence();
-  }
+  // lemma HBandMBwithSigMatchSequence(header: Msg.Header, hbSeq: seq<uint8>, frames: seq<MessageBody.Frame>, signature: seq<uint8>, message: seq<uint8>)
+  //   requires forall frame: MessageBody.Frame | frame in frames :: frame.Valid()
+  //   requires |message| >= |hbSeq| + |header.auth.iv + header.auth.authenticationTag| + |MessageBody.FramesToSequence(frames)|
+  //   requires exists headerLength, frameLength | 0 <= headerLength <= frameLength < |message| ::
+  //     && HeaderBySequence(header, hbSeq, message[..headerLength])
+  //     && FramesBySequence(frames, message[headerLength..frameLength])
+  //     && SignatureBySequence(signature, message[frameLength..])
+  //   ensures |signature| < UINT16_LIMIT &&
+  //     message == hbSeq + header.auth.iv + header.auth.authenticationTag + MessageBody.FramesToSequence(frames) + UInt16ToSeq(|signature| as uint16) + signature;
+  // {
+  //   reveal HeaderBySequence(), FramesBySequence(), SignatureBySequence();
+  // }
 
   lemma UpperBoundRemv(sequence: seq<uint8>, lo: int)
     requires 0 <= lo <= |sequence|
@@ -659,10 +664,10 @@ module {:extern "EncryptDecrypt"} EncryptDecrypt {
 
   }
 
-  predicate DataIsFramed(sequence: seq<uint8>)
-  {
-    exists i, header, hbSeq | 0 <= i <= |sequence| :: HeaderBySequence(header, hbSeq, sequence[..i])
-  }
+  // predicate DataIsFramed(sequence: seq<uint8>)
+  // {
+  //   exists i, header, hbSeq | 0 <= i <= |sequence| :: HeaderBySequence(header, hbSeq, sequence[..i])
+  // }
 
   lemma LemmaESDKAlgorithmSuiteIdImpliesEquality(
     esdkId: SerializableTypes.ESDKAlgorithmSuiteId,
